cp-adv/cp.dfy
@@ -15,9 +15,97 @@ method ArrayFromSeq<A>(s: seq<A>) returns (a: array<A>)
 
 method {:main} Main(ghost env: HostEnvironment?)
   requires env != null && env.Valid() && env.ok.ok();
-  modifies env.ok
-  modifies env.files
-{
+  requires |env.constants.CommandLineArgs()|>=3
+  requires if env.constants.CommandLineArgs()[2] in env.files.state() then |env.constants.CommandLineArgs()| >= 4 && env.constants.CommandLineArgs()[3] == "-o"[..] else |env.constants.CommandLineArgs()| >= 3
+  requires env.constants.CommandLineArgs()[1] in env.files.state()
 
-    print "done!\n";
+
+  modifies env.ok
+  modifies env.files 
+  ensures env.ok.ok()  ==> env.constants.CommandLineArgs()[2] in env.files.state();
+  ensures env.ok.ok() ==> env.constants.CommandLineArgs()[1] in env.files.state()
+  ensures env.ok.ok()  ==> var copy := env.constants.CommandLineArgs()[2];
+                          var original :=env.constants.CommandLineArgs()[1];
+          env.files.state() == old(env.files.state())[copy:= old(env.files.state())[original]];
+  ensures env.ok.ok() ==> copyFile(env.constants.CommandLineArgs()[1],env.constants.CommandLineArgs()[2],env); 
+  {
+
+  var numArgs :=env.constants.NumCommandLineArgs(env);
+  if(numArgs<3){
+     print("Not enough arguments, it requires 2");
+  }
+  var override := false;
+  var bufferSize,writeBufferSize:=0,0;
+  var sucessLen := false;
+  var original:= env.constants.GetCommandLineArg(1,env);   
+  var copy :=env.constants.GetCommandLineArg(2,env);
+  if(numArgs>=4){
+    var arg := env.constants.GetCommandLineArg(3,env);
+    override := arg[..] == "-o"[..];
+  }
+   assert override ==> |env.constants.CommandLineArgs()| >= 4 && env.constants.CommandLineArgs()[3] == "-o"[..];
+  var OriginalExist :=FileStream.FileExists(original,env);
+  
+  if(!OriginalExist){
+    print("Original file not found...");
+  }
+  assert OriginalExist ==> old(env.constants.CommandLineArgs())[1] in env.files.state();
+  var CopyExist := FileStream.FileExists(copy,env);
+  assert CopyExist ==> old(env.constants.CommandLineArgs())[2] in env.files.state();
+  if(CopyExist && !override){
+    print("Add -o if you want to override");  
+  }
+
+  if(OriginalExist && CopyExist && override) {
+    sucessLen,bufferSize := FileStream.FileLength(original,env); 
+  }else if(OriginalExist && !CopyExist){
+    sucessLen,bufferSize := FileStream.FileLength(original,env);
+  }
+  var originalStream, copyStream;
+  var successOriginal,successCopy:=false,false;
+  var successRead,successWrite := false,false;
+   var successClose,successCloseCopy := false,false;
+  if(sucessLen && (!CopyExist || (CopyExist && override))){
+    var buffer := new  byte[bufferSize];
+    successOriginal,originalStream := FileStream.Open(original,env);
+    if(successOriginal){
+      successCopy,copyStream := FileStream.Open(copy,env);
+      if(successCopy){
+        successRead := originalStream.Read(0,buffer,0,bufferSize);
+        assert env.ok.ok() ==> old(env.files.state())[original[..]] == buffer[..];
+        if(successRead){
+          successWrite := copyStream.Write(0,buffer,0,bufferSize); 
+          assert env.ok.ok() ==> env.files.state()[copy[..]] == buffer[..];
+          assert env.ok.ok() ==> env.files.state() == old(env.files.state())[copy[..]:=buffer[..]] ; 
+          if(successWrite){
+            successClose := originalStream.Close();
+            if(successClose){
+              successCloseCopy := copyStream.Close();        
+              if(successCloseCopy){
+                print("DONE!");
+              }
+            }
+          }
+        }
+      }
+    }
+  }
+  
+  if(!successCloseCopy && OriginalExist && !CopyExist){
+     print("Something went wrong");
+  }
+   
+  } 
+  
+predicate copyFile(original : seq<char>,copy : seq<char>, env: HostEnvironment)
+reads env.ok
+reads env
+reads env.files
+requires  env.Valid() 
+requires env.ok.ok()
+requires original in env.files.state()
+requires copy in env.files.state()
+{
+  env.files.state()[original] == env.files.state()[copy]
 }
+
